start of mem

src/llvm.i.dfy
@@ -11,18 +11,33 @@ module LLVM_def {
 
     datatype Value = uint8 | uint16 | uint32 | uint64 | uint128
 
+    //Memory
+    datatype mb = Mb(sz:int, b:byte)
+    datatype mptr = Mptr(blk:string,ofs:int,idx:int)
+    datatype munit = addr
+    datatype memoryCell = mb | mptr | munit
+
+    type memmap = map<addr, memoryCell>
 
     datatype state = State(
         lvs:map<LocalVar, Value>,
         gvs:map<GlobalVar, Value>,
+        m:memmap,
         ok:bool)
 
+    function{:axiom} TheValidAddresses(): set<addr>
+    predicate{:opaque} ValidMemState(s:memmap)
+    {
+        // regular mem
+        (forall m:addr :: m in TheValidAddresses() <==> m in s)    
+    }
 
     predicate State_Init(s:state)
     {
         s.ok 
         && |s.lvs| == 0
-        && |s.gvs| == 0    
+        && |s.gvs| == 0
+        && ValidMemState(s.m)    
     }
 
     // predicate Valid_State(s:State)
